Quicksort.v
@@ -1,3 +1,5 @@
+Add Rec LoadPath "/home/zeimer/Code/Coq".
+
 Require Import Sort.
 
 Theorem filter_length : forall (A : Type) (f : A -> bool) (l : list A),
@@ -52,14 +54,14 @@ Eval compute in (qs' natle testl).
 
 Require Import Coq.Init.Wf.
 
-Inductive qsDom (A : LinDec) : list A -> Type :=
-    | qsDom0 : qsDom A nil
+Inductive qsDom {A : LinDec} : list A -> Type :=
+    | qsDom0 : qsDom nil
     | qsDom1 : forall (h : A) (t : list A),
-        qsDom A (filter (fun x : A => leqb x h) t) ->
-        qsDom A (filter (fun x : A => negb (leqb x h)) t) ->
-        qsDom A (h :: t).
+        qsDom (filter (fun x : A => leqb x h) t) ->
+        qsDom (filter (fun x : A => negb (leqb x h)) t) ->
+        qsDom (h :: t).
 
-Fixpoint qs3' (A : LinDec) (l : list A) (dom : qsDom A l) : list A :=
+Fixpoint qs3' (A : LinDec) (l : list A) (dom : qsDom l) : list A :=
 match dom with
     | qsDom0 => nil
     | qsDom1 h t dom1 dom2 =>
@@ -67,11 +69,10 @@ match dom with
         qs3' A (filter (fun x : A => negb (leqb x h)) t) dom2
 end.
 
-Theorem all_qsDom : forall (A : LinDec) (l : list A), qsDom A l.
+Theorem all_qsDom : forall (A : LinDec) (l : list A), qsDom l.
 Proof.
-  intro.
-  apply well_founded_induction_type with (fun l1 l2 => length l1 < length l2).
-    eapply well_founded_lt_compat. eauto.
+  intro. apply well_founded_induction_type with lengthOrder.
+    apply lengthOrder_wf.
     intros. destruct x as [| h t]; constructor.
       apply X. simpl. unfold lt. apply le_n_S. apply filter_length.
       apply X. simpl. unfold lt. apply le_n_S. apply filter_length.
@@ -81,3 +82,39 @@ Definition qs3 (A : LinDec) (l : list A) : list A :=
     qs3' A l (all_qsDom A l).
 
 Eval compute in qs3 natle testl.
+
+(* Tried to prove that quicksort gives a permutation, but failed. *)
+(*Lemma nb_occ_app : forall (A : LinDec) (l1 l2 : list A) (x : A),
+    nb_occ A x (l1 ++ l2) = nb_occ A x (l2 ++ l1).
+Proof.
+  induction l1 as [| h t]; induction l2 as [| h' t']; simpl;
+  intros; repeat rewrite app_nil_r; auto. simpl in *.
+  case_eq (LinDec_eq x h); case_eq (LinDec_eq x h'); intros.
+  f_equal. assert (h = h'). unfold LinDec_eq in H. 
+    
+
+Lemma perm_app : forall (A : LinDec) (l1 l2 : list A),
+    perm A (l1 ++ l2) (l2 ++ l1).
+Proof.
+  induction l1 as [| h t].
+    simpl. intro. rewrite app_nil_r. apply perm_refl.
+    simpl. induction l2 as [| h' t'].
+      simpl. rewrite app_nil_r. apply perm_refl.
+      simpl. SearchAbout perm. Print perm.
+
+Lemma perm_lemma : forall (A : LinDec) (h : A) (t l1 l2 : list A),
+    perm A t (l1 ++ l2) -> perm A (h :: t) (l1 ++ h :: l2).
+Proof.
+  intros.
+
+Program Fixpoint qs' (A : LinDec) (l : list A) {measure (length l)}
+    : {l' : list A | perm A l l'} :=
+match l with
+    | nil => nil
+    | h :: t => qs' A (filter (fun x : A => leqb x h) t) ++ [h]
+             ++ qs' A (filter (fun x : A => negb (leqb x h)) t)
+end.
+Next Obligation. constructor. Qed.
+Next Obligation. simpl. unfold lt. auto. Qed.
+Next Obligation. simpl. unfold lt. auto. Qed.
+Next Obligation. *)
